Add very basic theorem about calling the demo contract

vyperDemoScript.sml
@@ -47,6 +47,89 @@ Definition demo_ast_def:
   ]
 End
 
+(* TODO: why doesn't this work later?
 val () = cv_trans_deep_embedding EVAL demo_ast_def;
+*)
+val () = cv_auto_trans demo_ast_def;
+
+val deployer = “0x42w: address”
+val contract = “0x0123w: address”
+
+Definition deploy_demo_def:
+  deploy_demo =
+  let deployer = ^deployer in
+  let addr = ^contract in
+  let goal_amount = 10 ** 18 in
+  let deploy_tx = transaction deployer addr "__init__" [IntV &goal_amount] 0 in
+    OUTL $ load_contract initial_machine_state deploy_tx demo_ast
+End
+
+val deploy_demo_pre_def = cv_auto_trans_pre deploy_demo_def;
+
+fun cv_eval_match pat tm = let
+  val t1 = find_term (can $ match_term pat) tm
+  val th = cv_eval t1
+in PURE_REWRITE_CONV [th] tm end
+
+Theorem deploy_demo_pre[cv_pre]:
+  deploy_demo_pre
+Proof
+  rw[deploy_demo_pre_def, load_contract_def]
+  \\ CONV_TAC(cv_eval_match“lookup_function _ _ _”)
+  \\ rw[]
+  \\ CONV_TAC(cv_eval_match“step_external_function _ _ _ _”)
+  \\ rw[]
+QED
+
+Theorem deploy_demo_eq = cv_eval “deploy_demo”
+
+Theorem demo_check_end_campaign_other:
+  tx = <| sender := addr; target := ^contract;
+          value := 0; args := [];
+          function_name := "end_campaign" |>
+  ==>
+  FST $ external_call deploy_demo tx =
+  if addr = ^deployer then INL NoneV
+  else INR "Assertion Failed: Only creator"
+Proof
+  rw[]
+  >- CONV_TAC cv_eval
+  \\ simp[external_call_def]
+  \\ rewrite_tac[Once deploy_demo_eq]
+  \\ qmatch_goalsub_abbrev_tac`contract src gbs`
+  \\ simp[external_call_contract_def]
+  \\ qunabbrev_tac`src`
+  \\ CONV_TAC(cv_eval_match “lookup_function _ _ _”)
+  \\ qmatch_goalsub_abbrev_tac`contract src gbs`
+  \\ simp[step_external_function_def]
+  \\ CONV_TAC(cv_eval_match “bind_arguments _ _”)
+  \\ simp[]
+  \\ CONV_TAC(cv_eval_match “initial_function_context _ _ _”)
+  \\ simp[Once step_stmt_till_exception_def]
+  \\ simp[Once initial_execution_context_def, exception_raised_def]
+  \\ simp[Once initial_execution_context_def]
+  \\ simp[Once step_stmt_def, set_stmt_def]
+  \\ simp[Once step_stmt_till_exception_def, exception_raised_def]
+  \\ simp[Once step_stmt_def, set_stmt_def]
+  \\ simp[step_expr_def]
+  \\ CONV_TAC(cv_eval_match “AssertK _ _”)
+  \\ simp[Once step_stmt_till_exception_def, exception_raised_def]
+  \\ simp[Once step_stmt_def, set_stmt_def]
+  \\ simp[step_expr_def]
+  \\ simp[Once step_stmt_till_exception_def, exception_raised_def]
+  \\ simp[Once step_stmt_def, set_stmt_def]
+  \\ simp[step_expr_def]
+  \\ qunabbrev_tac`gbs`
+  \\ CONV_TAC(cv_eval_match “FLOOKUP _ _”)
+  \\ simp[evaluate_builtin_def]
+  \\ qmatch_goalsub_abbrev_tac`contract src gbs`
+  \\ qmatch_goalsub_abbrev_tac`BoolV b`
+  \\ `b = (addr = 66w)` by cheat (* word_to_bytes_word_of_bytes_20 *)
+  \\ gvs[Abbr`b`]
+  \\ simp[Once step_stmt_till_exception_def, exception_raised_def]
+  \\ simp[Once step_stmt_def, set_stmt_def, raise_def]
+  \\ simp[Once step_stmt_till_exception_def, exception_raised_def]
+  \\ CONV_TAC cv_eval
+QED
 
 val () = export_theory();
